Constant propagation inside expression.

Leanr/Expression.lean
@@ -15,6 +15,9 @@ def Expression.eval {p : ℕ} (e : Expression p) (env : String → ZMod p): ZMod
   | .add e1 e2 => e1.eval env + e2.eval env
   | .mul e1 e2 => e1.eval env * e2.eval env
 
+def Expression.equivalent {p : ℕ} (e1 e2 : Expression p) : Prop :=
+  ∀ env : String → ZMod p, e1.eval env = e2.eval env
+
 def Expression.substitute {p : ℕ} (e : Expression p) (x : String) (v : ZMod p) : Expression p :=
   match e with
   | .const n => .const n
@@ -22,3 +25,41 @@ def Expression.substitute {p : ℕ} (e : Expression p) (x : String) (v : ZMod p)
   | .add e1 e2 => .add (e1.substitute x v) (e2.substitute x v)
   | .mul e1 e2 => .mul (e1.substitute x v) (e2.substitute x v)
 
+def Expression.simplify {p : ℕ} (e : Expression p) : Expression p :=
+  match e with
+  | .const n => .const n
+  | .var x => .var x
+  | .add e1 e2 =>
+    let e1 := e1.simplify
+    let e2 := e2.simplify
+    match e1, e2 with
+    -- | .const 0, _ => e2
+    -- | _, .const 0 => e1
+    | .const n1, .const n2 => .const (n1 + n2)
+    | _, _ => .add e1 e2
+  | .mul e1 e2 =>
+    let se1 := e1.simplify
+    let se2 := e2.simplify
+    match se1, se2 with
+    | .const n1, .const n2 => .const (n1 * n2)
+    -- | .const 0, _ => .const 0
+    -- | _, .const 0 => .const 0
+    -- | .const 1, _ => se2
+    -- | _, .const 1 => se1
+    | _, _ => .mul se1 se2
+
+-- Expression.simplify does not modify the semantics of the expression.
+theorem simplify_correct {p : ℕ} (e : Expression p) :
+  Expression.equivalent e e.simplify := by
+  intro env
+  induction e with
+  | const n => simp [Expression.eval, Expression.simplify]
+  | var x => simp [Expression.eval, Expression.simplify]
+  | add e1 e2 ih1 ih2 =>
+      cases h1 : Expression.simplify e1 <;>
+      cases h2 : Expression.simplify e2 <;>
+      simp [Expression.eval, Expression.simplify, h1, h2, ih1, ih2]
+  | mul e1 e2 ih1 ih2 =>
+      cases h1 : Expression.simplify e1 <;>
+      cases h2 : Expression.simplify e2 <;>
+      simp [Expression.eval, Expression.simplify, h1, h2, ih1, ih2]
